Progress on well-formedness of [FV]s.

examples/ghc/theories/FV.v
@@ -1,6 +1,9 @@
 Require Import Core.
 Require Import FV.
 Require Import Proofs.ContainerAxioms.
+Require Import Proofs.VarSet.
+Require Import Proofs.VarSetFSet.
+Require Import Proofs.Var.
 
 Require Import Coq.Lists.List.
 Require Import Coq.Bool.Bool.
@@ -10,16 +13,51 @@ Import GHC.Base.ManualNotations.
 
 Set Bullet Behavior "Strict Subproofs".
 
-Axiom realUnique_eq : forall x y,
-    (x == y) = (realUnique x == realUnique y).
+Reserved Notation "A ⊢ B" (at level 70, no associativity).
+Inductive Denotes : VarSet -> FV -> Prop :=
+| DenotesVarSet : forall vs fv,
+    (forall f in_scope vs' l,
+        extendVarSetList emptyVarSet l = vs' ->
+        extendVarSetList emptyVarSet (fst (fv f in_scope (l, vs'))) =
+        snd (fv f in_scope (l, vs')) /\
+        snd (fv f in_scope (l, vs')) =
+        unionVarSet (minusVarSet (filterVarSet f vs) in_scope) vs') ->
+    vs ⊢ fv
+where "A ⊢ B" := (Denotes A B).
 
-(** For simplicity, only consider deletion for now. *)
-Definition WF_fv (fv : FV) : Prop :=
-  forall f bs l vs,
-    (forall x, elemVarSet x vs && elemVarSet x bs = false) ->
-    let '(l', vs') := fv f bs (l, vs) in
-    (forall x, elemVarSet x bs = true -> elemVarSet x vs' = false) /\
-    (bs = emptyVarSet -> vs = vs').
+Ltac unfold_uniqSet :=
+  match goal with
+  | |- context[match ?a with UniqSet.Mk_UniqSet _ => _ end] =>
+    destruct a
+  end.
+
+Ltac unfold_UFM :=
+  match goal with
+  | |- context[match ?a with UniqFM.UFM _ => _ end] =>
+    destruct a
+  end.
+
+Ltac unfold_fv := simpl; unfold_uniqSet; unfold_UFM.
+
+Ltac destruct_match :=
+  match goal with
+  | |- context[match ?a with _ => _ end] =>
+    let H := fresh "Hmatch" in
+    destruct a eqn:H
+  end.
+
+Theorem Denotes_fvVarSet : forall m fv f in_scope l vs,
+    m ⊢ fv ->
+    extendVarSetList emptyVarSet l = vs ->
+    snd (fv f in_scope (l, vs)) =
+    unionVarSet (minusVarSet (filterVarSet f m) in_scope) vs.
+Proof.
+  intros. inversion H.
+  specialize (H1 f in_scope vs l ); subst.
+  apply H1; reflexivity.
+Qed.
+
+Definition WF_fv (fv : FV) : Prop := exists vs, vs ⊢ fv.
 
 Lemma elemVarSet_neq :
   forall x y vs,
@@ -32,7 +70,7 @@ Proof.
   unfold UniqFM.elemUFM; destruct u. intro H.
   rewrite member_eq with (k':=(Unique.getWordKey (Unique.getUnique x))) in H.
   - rewrite H. discriminate.
-  - simpl. rewrite realUnique_eq in H1. cbn in H1.
+  - simpl. rewrite <- realUnique_eq in H1. cbn in H1.
     apply Nat.eqb_eq in H1. rewrite H1. cbn. apply N.eqb_refl.
 Qed.
 
@@ -47,33 +85,86 @@ Proof.
   unfold UniqFM.addToUFM, UniqFM.elemUFM. destruct u. intros Hmem.
   rewrite member_insert. apply orb_false_iff; split; [ | assumption].
   apply not_true_is_false. intro.
-  cbn in H0. apply N.eqb_eq in H0. apply Nat2N.inj in H0.
-  rewrite <- Nat.eqb_eq, <- realUnique_eq in H0. rewrite H in H0. discriminate.
-Qed.  
+  cbn in H0. cbn in H. apply N.eqb_eq in H0. apply Nat2N.inj in H0.
+  rewrite <- Nat.eqb_eq in H0. rewrite H in H0. discriminate.
+Qed.
+
+Lemma empty_FV_WF :
+  WF_fv emptyFV.
+Proof.
+  unfold WF_fv. exists emptyVarSet. constructor; intros; subst.
+  unfold_fv. rewrite difference_nil_l, <- mkVarSet_extendVarSetList.
+  unfold_fv. intuition. do 2 f_equal. symmetry. apply union_nil_r.
+Qed.
 
 Lemma unit_FV_WF :
   forall x, WF_fv (unitFV x).
 Proof.
-  unfold WF_fv; intros.
-  destruct (unitFV x f bs (l, vs)) eqn:Hfv; intros.
-  unfold unitFV in Hfv.
-  destruct (elemVarSet x bs) eqn:Hin.
-  - inversion Hfv; subst. split; [| reflexivity].
-    intros x0 H'. specialize (H x0).
-    apply andb_false_elim in H; destruct H; [assumption | congruence].
-  - destruct (elemVarSet x vs) eqn:Hin'.
-    + inversion Hfv; subst. split; [| reflexivity].
-      intros. specialize (H x0).
-      apply andb_false_elim in H; destruct H; [assumption | congruence].
-    + destruct (f x) eqn:Hf.
-      * inversion Hfv; subst. split.
-        -- intros. specialize (H x0); apply andb_false_elim in H.
-           destruct H; try congruence.
-           apply (elemVarSet_neq _ _ _ H0) in Hin.
-           apply elemVarSet_extendVarSet; try assumption.
-        -- inversion Hfv; subst; assumption.
+  intros. unfold WF_fv.
+  exists (unitVarSet x).
+  constructor; intros; subst. simpl.
+  destruct_match; simpl.
+  - unfold_fv. rewrite <- mkVarSet_extendVarSetList.
+    destruct_match; unfold_fv; repeat f_equal.
+    + admit. (* should be true *)
+    + rewrite difference_nil_l, union_nil_r. intuition.
+  - destruct_match; simpl.
+    + unfold_fv. rewrite <- mkVarSet_extendVarSetList.
+      destruct_match; unfold_fv; repeat f_equal.
+      * admit.
+      * rewrite difference_nil_l, union_nil_r. intuition.
+    + destruct_match.
+      * unfold_fv. rewrite <- mkVarSet_extendVarSetList.
+        unfold_fv. simpl. repeat f_equal. admit.
+      * unfold_fv. rewrite <- mkVarSet_extendVarSetList.
+        unfold_fv. repeat f_equal.
+        rewrite difference_nil_l, union_nil_r. intuition.
+Admitted.
+
+Ltac unfold_WF :=
+  repeat match goal with
+  | [ H : WF_fv ?fv |- _] =>
+    let vs := fresh "vs" in
+    let Hd := fresh "Hdenotes" in
+    inversion H as [vs Hd]; inversion Hd; subst; clear H
+  | [ |- WF_fv ?fv ] =>
+    unfold WF_fv
+  end.
+
+Lemma filter_FV_WF : forall f x,
+    WF_fv x -> WF_fv (filterFV f x).
+Proof.
+  intros. unfold_WF.
+  exists (filterVarSet f vs). constructor; intros.
+  unfold filterFV.
+  specialize (H0 (fun v : Var => f0 v && f v) in_scope vs' l H).
+  destruct H0. intuition.
+  rewrite H1. rewrite <- filterVarSet_comp. reflexivity.
 Qed.
 
+Lemma del_FV_WF : forall fv v,
+    WF_fv fv -> WF_fv (delFV v fv).
+Proof.
+  intros. unfold_WF.
+  exists (delVarSet vs v). constructor; intros. unfold delFV.
+  specialize (H0 f (extendVarSet in_scope v) vs' l H).
+  destruct H0. intuition. rewrite H1.
+  (* Seems true. Need theorems from [VarSet]. *)
+Admitted.
+
+Lemma union_FV_WF : forall fv fv',
+    WF_fv fv -> WF_fv fv' -> WF_fv (unionFV fv fv').
+Proof.
+  intros. unfold_WF.
+  exists (unionVarSet vs vs0). constructor; intros.
+  unfold unionFV.
+  specialize (H1 f in_scope vs' l H). destruct H1.
+  remember (fv' f in_scope (l, vs')) as vs_mid.
+  specialize (H0 f in_scope (snd vs_mid) (fst vs_mid) H1); destruct H0.
+  replace vs_mid with (fst vs_mid, snd vs_mid); [| destruct vs_mid; reflexivity].
+  intuition. rewrite H3. rewrite H2.
+Admitted.
+  
 Lemma union_empty_l : forall fv, FV.unionFV FV.emptyFV fv = fv.
 Proof. reflexivity. Qed.
 
